---
description: |
  Joint monomorphisms.
---
<!--
```agda
open import Cat.Diagram.Product.Indexed
open import Cat.Diagram.Product
open import Cat.Prelude

import Cat.Reasoning
```
-->
```agda
module Cat.Morphism.Joint.Mono {o ℓ} (C : Precategory o ℓ) where
```

<!--
```agda
open Cat.Reasoning C
```
-->

# Joint monomorphisms {defines="joint-monomorphism"}

:::{.definition #jointly-monic}
A pair of morphisms $f : \cC(X,Y)$ and $g : \cC(X,Z)$ are **jointly monic**
if for every $h, k : \cC(A,X)$, $h = k$ if $f \circ h = f \circ k$ and
$g \circ h = g \circ k$.
:::

```agda
is-jointly-monic : ∀ {x y z} → Hom x y → Hom x z → Type (o ⊔ ℓ)
is-jointly-monic {x = x} f g =
  ∀ {a} → (h k : Hom a x) → f ∘ h ≡ f ∘ k → g ∘ h ≡ g ∘ k → h ≡ k
```

:::{.definition #jointly-monic-family}
More generally, an $I$-indexed family of morphisms $f_{i} : \cC(X, Y_{i})$
is a **jointly monic family** if for every $h, k : \cC(A,X)$, $h = k$ if
$f_{i} \circ h = f_{i} \circ k$ for every $i : I$.
:::

```agda
is-jointly-monic-fam
  : ∀ {ℓ'} {I : Type ℓ'}
  → {x : Ob} {yᵢ : I → Ob}
  → (fᵢ : ∀ i → Hom x (yᵢ i))
  → Type (o ⊔ ℓ ⊔ ℓ')
is-jointly-monic-fam {x = x} fᵢ =
  ∀ {a} → (h k : Hom a x) → (∀ i → fᵢ i ∘ h ≡ fᵢ i ∘ k) → h ≡ k
```

## Joint monomorphisms and products

If $\cC$ has [[products]], then a pair of morphisms $f : \cC(X,Y)$, $g : \cC(X,Z)$
is jointly monic if and only if $\langle f , g \rangle : \cC(X,Y \times Z)$
is [[monic]].

```agda
module _ (all-products : has-products C) where
  open Binary-products C all-products
```

The forward direction follows from a short calculation.

```agda
  ⟨⟩-monic→jointly-monic
    : ∀ {x y z} {f : Hom x y} {g : Hom x z}
    → is-monic ⟨ f , g ⟩
    → is-jointly-monic f g
  ⟨⟩-monic→jointly-monic {f = f} {g = g} ⟨f,g⟩-mono h k p q =
    ⟨f,g⟩-mono h k $
      ⟨ f , g ⟩ ∘ h     ≡⟨ ⟨⟩∘ h ⟩
      ⟨ f ∘ h , g ∘ h ⟩ ≡⟨ ap₂ ⟨_,_⟩ p q ⟩
      ⟨ f ∘ k , g ∘ k ⟩ ≡˘⟨ ⟨⟩∘ k ⟩
      ⟨ f , g ⟩ ∘ k     ∎
```

The reverse direction is a bit trickier, but only just. Suppose that
$f, g$ are jointly monic, and let $h, k : \cC(A,X)$ such that

$$\langle f , g \rangle \circ h = \langle f , g \rangle \circ k$$

Our goal is to show that $h = k$. As $f$ and $g$ are jointly monic,
it suffices to show that $f \circ h = f \circ k$ and $g \circ h = g \circ k$.
We can re-arrange our hypothesis to get that

$$\langle f \circ h , g \circ h \rangle = \langle f \circ k , g \circ k \rangle$$

If we apply first and second projections to this equation, then we get
exactly the pair of equalities that we were looking for.

```agda
  jointly-monic→⟨⟩-monic
    : ∀ {x y z} {f : Hom x y} {g : Hom x z}
    → is-jointly-monic f g
    → is-monic ⟨ f , g ⟩
  jointly-monic→⟨⟩-monic {f = f} {g = g} fg-joint-mono h k p =
    fg-joint-mono h k (by-π₁ ⟨fh,gh⟩=⟨fk,gk⟩) (by-π₂ ⟨fh,gh⟩=⟨fk,gk⟩)
    where
      ⟨fh,gh⟩=⟨fk,gk⟩ : ⟨ f ∘ h , g ∘ h ⟩ ≡ ⟨ f ∘ k , g ∘ k ⟩
      ⟨fh,gh⟩=⟨fk,gk⟩ =
        ⟨ f ∘ h , g ∘ h ⟩ ≡˘⟨ ⟨⟩∘ h ⟩
        ⟨ f , g ⟩ ∘ h     ≡⟨ p ⟩
        ⟨ f , g ⟩ ∘ k     ≡⟨ ⟨⟩∘ k ⟩
        ⟨ f ∘ k , g ∘ k ⟩ ∎
```

This result provides the main motivation for joint monomorphisms. Namely,
joint monos let us talk about [[subobjects]] of products, even when those products
may not exist. Put another way, joint monos offer an alternative characterisation
of relations internal to $\cC$ that works even when $\cC$ lacks products.

Joint monos are also slightly more ergonomic than subobjects of products.
Typically, if we want to prove that some $R \mono X \times Y$ is monic,
then our first step is to invoke the universal property of $R$: joint
monos factor out this first step into the definition!

## Jointly monic families and indexed products

We can obtain a similar result for jointly monic families and [[indexed products]]:
if $\cC$ has $I$-indexed products, then a family of morphisms $f_{i} : \cC(X, Y_{i})$
is jointly monic if and only if the universal map $\prod f_{i} : \cC(X, \prod Y_{i})$
is monic.

```agda
module _ {ℓ} {I : Type ℓ} (indexed-products : has-products-indexed-by C I) where
  private module ∏ {xᵢ : I → Ob} = Indexed-product (indexed-products xᵢ)

  tuple-monic→jointly-monic-fam
    : ∀ {x} {yᵢ : I → Ob}
    → {fᵢ : ∀ i → Hom x (yᵢ i)}
    → is-monic (∏.tuple fᵢ)
    → is-jointly-monic-fam fᵢ

  jointly-monic-fam→tuple-monic
    : ∀ {x} {yᵢ : I → Ob}
    → {fᵢ : ∀ i → Hom x (yᵢ i)}
    → is-jointly-monic-fam fᵢ
    → is-monic (∏.tuple fᵢ)
```

<details>
<summary>The proofs are almost identical to the non-indexed case, so we
omit the details in the interest of brevity.
</summary>

```agda
  tuple-monic→jointly-monic-fam {yᵢ = yᵢ} {fᵢ = fᵢ} tuple-mono h k p =
    tuple-mono h k $
      ∏.tuple fᵢ ∘ h           ≡⟨ tuple∘ C yᵢ (indexed-products yᵢ) fᵢ ⟩
      ∏.tuple (λ i → fᵢ i ∘ h) ≡⟨ ap ∏.tuple (funext p) ⟩
      ∏.tuple (λ i → fᵢ i ∘ k) ≡˘⟨ tuple∘ C yᵢ (indexed-products yᵢ) fᵢ ⟩
      ∏.tuple fᵢ ∘ k           ∎

  jointly-monic-fam→tuple-monic {yᵢ = yᵢ} {fᵢ = fᵢ} fᵢ-joint-mono h k p =
    fᵢ-joint-mono h k λ i →
      fᵢ i ∘ h               ≡⟨ pushl (sym ∏.commute) ⟩
      ∏.π i ∘ ∏.tuple fᵢ ∘ h ≡⟨ ap (∏.π i ∘_) p ⟩
      ∏.π i ∘ ∏.tuple fᵢ ∘ k ≡⟨ pulll ∏.commute ⟩
      fᵢ i ∘ k               ∎
```
</details>

If we apply the same line of reasoning that we used at the end of the
previous section, we will notice that $I$-indexed jointly monic families
are $I$-ary relations internal to $\cC$.

## Closure properties of joint monos

If $f, g$ are jointly monic and $h$ is monic, then
$f \circ h$ and $g \circ h$ are jointly monic.

```agda
jointly-monic-∘
  : ∀ {w x y z} {f : Hom x y} {g : Hom x z} {h : Hom w x}
  → is-jointly-monic f g
  → is-monic h
  → is-jointly-monic (f ∘ h) (g ∘ h)
jointly-monic-∘ {h = h} fg-joint-mono h-mono k₁ k₂ p q =
  h-mono k₁ k₂ $
  fg-joint-mono (h ∘ k₁) (h ∘ k₂)
    (assoc _ _ _ ·· p ·· sym (assoc _ _ _))
    (assoc _ _ _ ·· q ·· sym (assoc _ _ _))
```

Moreover, if $f \circ h$ and $g \circ h$ are jointly monic, then
$h$ is monic.

```agda
jointly-monic-cancell
  : ∀ {w x y z} {f : Hom x y} {g : Hom x z} {h : Hom w x}
  → is-jointly-monic (f ∘ h) (g ∘ h)
  → is-monic h
jointly-monic-cancell fgh-joint-mono k₁ k₂ p =
  fgh-joint-mono k₁ k₂ (extendr p) (extendr p)
```

We get a similar pair of results for jointly monic families.

```agda
jointly-monic-fam-∘
  : ∀ {ℓ'} {I : Type ℓ'} {x y} {zᵢ : I → Ob}
  → {fᵢ : ∀ i → Hom y (zᵢ i)} {g : Hom x y}
  → is-jointly-monic-fam fᵢ
  → is-monic g
  → is-jointly-monic-fam (λ i → fᵢ i ∘ g)
jointly-monic-fam-∘ {g = g} fᵢ-joint-mono g-mono k₁ k₂ p =
  g-mono k₁ k₂ $
  fᵢ-joint-mono (g ∘ k₁) (g ∘ k₂) λ i →
    assoc _ _ _ ·· p i ·· sym (assoc _ _ _)

jointly-monic-fam-cancell
  : ∀ {ℓ'} {I : Type ℓ'} {x y} {zᵢ : I → Ob}
  → {fᵢ : ∀ i → Hom y (zᵢ i)} {g : Hom x y}
  → is-jointly-monic-fam (λ i → fᵢ i ∘ g)
  → is-monic g
jointly-monic-fam-cancell fᵢg-joint-mono k₁ k₂ p =
  fᵢg-joint-mono k₁ k₂ λ i → extendr p
```

If either of $f : \cC(X,Y)$ or $g : \cC(X,Z)$ are monic, then
$f$ and $g$ are jointly monic.

```agda
left-monic→jointly-monic
  : ∀ {x y z} {f : Hom x y} {g : Hom x z}
  → is-monic f
  → is-jointly-monic f g
left-monic→jointly-monic f-mono k₁ k₂ p q =
  f-mono k₁ k₂ p

right-monic→jointly-monic
  : ∀ {x y z} {f : Hom x y} {g : Hom x z}
  → is-monic g
  → is-jointly-monic f g
right-monic→jointly-monic g-mono k₁ k₂ p q =
  g-mono k₁ k₂ q
```

Similarly, if any component of a family of maps $f_{i} : \cC(X,Y_{i})$
is monic, then $f_{i}$ is a jointly monic family.

```agda
monic→jointly-monic-fam
  : ∀ {ℓ'} {I : Type ℓ'} {x} {yᵢ : I → Ob}
  → {fᵢ : ∀ i → Hom x (yᵢ i)}
  → (i : I) → is-monic (fᵢ i)
  → is-jointly-monic-fam fᵢ
monic→jointly-monic-fam i fᵢ-monic k₁ k₂ p =
  fᵢ-monic k₁ k₂ (p i)
```

The previous result has an easy generalization: if $f_{j} : \cC(X,Y_{j})$
is a family of morphisms such $f_{j}$ is jointly monic when restricted
along a map $\sigma : I \to J$, then $f_{j}$ is jointly monic.

```agda
restrict-jointly-monic-fam
  : ∀ {ℓ' ℓ''} {I : Type ℓ'} {J : Type ℓ''}
  → ∀ {x} {yⱼ : J → Ob} {fⱼ : ∀ j → Hom x (yⱼ j)}
  → (σ : I → J)
  → is-jointly-monic-fam (λ i → fⱼ (σ i))
  → is-jointly-monic-fam fⱼ
restrict-jointly-monic-fam σ fⱼ-joint-mono k₁ k₂ p =
  fⱼ-joint-mono k₁ k₂ (λ j → p (σ j))
```

If $f$ is jointly monic with itself, then $f$ is monic. Moreover, if
the constant family $\lam i \to f$ is jointly monic, then $f$ is monic.

```agda
self-jointly-monic→monic
  : ∀ {x y} {f : Hom x y}
  → is-jointly-monic f f
  → is-monic f
self-jointly-monic→monic f-joint-monic k₁ k₂ p =
  f-joint-monic k₁ k₂ p p

self-jointly-monic-fam→monic
  : ∀ {ℓ'} {I : Type ℓ'} {x y} {f : Hom x y}
  → is-jointly-monic-fam (λ (i : I) → f)
  → is-monic f
self-jointly-monic-fam→monic f-joint-mono k₁ k₂ p =
  f-joint-mono k₁ k₂ (λ _ → p)
```

## Joint monos via representability

Like most things categorical, joint monos admit a definition via
representability: $f : \cC(X,Y)$ and $g : \cC(X,Z)$ are jointly monic
if and only if the map $\cC(A,X) \to \cC(A,Y) \times \cC(A,Z)$ induced
by postcomposition is an [[embedding]].

```agda
jointly-monic→postcomp-embedding
  : ∀ {x y z} {f : Hom x y} {g : Hom x z}
  → is-jointly-monic f g
  → ∀ {a} → is-embedding {B = Hom a y × Hom a z} (λ h → f ∘ h , g ∘ h)
jointly-monic→postcomp-embedding fg-joint-mono =
  injective→is-embedding! λ {k₁} {k₂} p →
    fg-joint-mono k₁ k₂ (ap fst p) (ap snd p)

postcomp-embedding→jointly-monic
  : ∀ {x y z} {f : Hom x y} {g : Hom x z}
  → (∀ {a} → is-embedding {B = Hom a y × Hom a z} (λ h → f ∘ h , g ∘ h))
  → is-jointly-monic f g
postcomp-embedding→jointly-monic {f = f} {g = g} postcomp-embed k₁ k₂ p q =
  ap fst $ postcomp-embed (f ∘ k₂ , g ∘ k₂) (k₁ , p ,ₚ q) (k₂ , refl)
```

More generally, $f_{i} : \cC(X,Y_{i})$ is a jointly monic family if and
only if the map $\cC(A,X) \to ((i : I) \to \cC(A,Y_{i}))$ induced by
postcomposition is an embedding.

```agda
jointly-monic-fam→postcomp-embedding
  : ∀ {ℓ} {I : Type ℓ} {x} {yᵢ : I → Ob}
  → {fᵢ : ∀ i → Hom x (yᵢ i)}
  → is-jointly-monic-fam fᵢ
  → ∀ {a} → is-embedding {B = (i : I) → Hom a (yᵢ i)} (λ g i → fᵢ i ∘ g)
jointly-monic-fam→postcomp-embedding fᵢ-joint-mono =
  injective→is-embedding! λ {k₁} {k₂} p →
    fᵢ-joint-mono k₁ k₂ (apply p)

postcomp-embedding→jointly-monic-fam
  : ∀ {ℓ} {I : Type ℓ} {x} {yᵢ : I → Ob}
  → {fᵢ : ∀ i → Hom x (yᵢ i)}
  → (∀ {a} → is-embedding {B = (i : I) → Hom a (yᵢ i)} (λ g i → fᵢ i ∘ g))
  → is-jointly-monic-fam fᵢ
postcomp-embedding→jointly-monic-fam {fᵢ = fᵢ} postcomp-embed k₁ k₂ p =
  ap fst $ postcomp-embed (λ i → fᵢ i ∘ k₂) (k₁ , funext p) (k₂ , refl)
```
