<!--
```agda
open import 1Lab.Reflection.Variables
open import 1Lab.Reflection
open import 1Lab.Path
open import 1Lab.Type

open import Data.Nat.Properties
open import Data.Fin.Base
open import Data.List hiding (lookup)
```
-->

```agda
module Data.Nat.Solver where
```

# The Nat solver

This module defines a solver for equations in the commutative semiring
of [natural numbers]. Our approach splits cleanly into 3 distinct parts:

[natural numbers]: Data.Nat.Base.html

- Horner normal forms for polynomials
- Evaluation of reflected terms into polynomials
- The reflection interface

## Horner normal forms

If we ignore the `suc`{.Agda} and `zero`{.Agda} constructors, and their
respective equations, the core problem at hand is trying to compute
normal forms for polynomials. Luckily, like most problems involving
polynomials, this has been thoroughly studied! There are many possible
normal forms to choose from, but the most useful for our task is *Horner
normal form*, as it admits a particularly nice inductive
characterization.

The core idea is that we can rewrite a (univariate) polynomial of the form
$$ a_0 + a_1 x + a_2 x^2 + a_3 x^3 + \cdots + a_n x^n $$
into the following form:
$$ a_0 + x ( a_1 + x ( a_2 + x ( a_3 + \cdots + x ( a_{n-1} + x a_n ) ) ) ) $$

However, we need _multivariate_ polynomials, not just univariate! To do
this, we exploit the isomorphism between $A[X_0, \cdots, X_n]$ and
$A[X_0][X_1]\cdots[X_n]$. This allows us to define the normal form of a
multivariate polynomial as (essentially) a product of univariate ones.

We start by defining the type of n-ary multivariate polynomials.

```agda
data Poly {a} (A : Type a) : Nat → Type a where
```

The first polynomial we define is the constant polynomial $c \in A[X_0]$.

```agda
  const : (c : A) → Poly A 0
```

Next, we define the 0 polynomial $0 \in A[X_0, \cdots, X_n]$. Note that
we do _not. include $A[X_0]$ here! This is important for ensuring that
our data type defines a (somewhat) _unique_ normal form. If we had
instead chosen `Poly A n`, we could represent the $0$ polynomial using
either `const 0` or `zerop`, which complicates matters somewhat.

```agda
  zerop  : ∀ {n} → Poly A (suc n)
```

Finally, we define both addition and multiplication by $X_0$ in one fell
swoop. This constructor represents the polynomial $p * X_0 + q$, where
$p \in A[X_0]\cdots[X_n]$, and $q \in A[X_1]\cdots[X_n]$.

This flipping of the index may seem confusing at first, but it serves an
important purpose: it makes evaluation _really_ easy! When evaluating,
we will need some environment `Vec A n` which assigns values to the
various indeterminates $X_i$. In the variable case, the indexing will
ensure that our environment is non-empty, whence we can use the tail of
the vector to evaluate `q`! In this sense, not only does this
constructor handle addition and multiplication by $X_0$, it _also_
handles weakening.

```agda
  _*X+_ : ∀ {n} → (p : Poly A (suc n)) → (q : Poly A n) → Poly A (suc n)
```

<!--
```agda
infixl 2 _*X+_

private variable
  a : Level
  A : Type a
  n : Nat

-- NOTE: These little helper lemmas become very useful, and make
-- some of the really involved proofs a lot less painful.
commute-inner : ∀ w x y z → (w + x) + (y + z) ≡ (w + y) + (x + z)
commute-inner w x y z =
  (w + x) + (y + z) ≡˘⟨ +-associative w x (y + z) ⟩
  w + (x + (y + z)) ≡⟨ ap (w +_) (+-associative x y z) ⟩
  w + ((x + y) + z) ≡⟨ ap (λ ϕ → w + (ϕ + z)) (+-commutative x y) ⟩
  w + (y + x + z)   ≡˘⟨ ap (w +_) (+-associative y x z) ⟩
  w + (y + (x + z)) ≡⟨  +-associative w y (x + z) ⟩
  (w + y) + (x + z) ∎

commute-last : ∀ x y z → (x * y) * z ≡ (x * z) * y
commute-last x y z =
  x * y * z   ≡⟨ *-associative x y z ⟩
  x * (y * z) ≡⟨ ap (x *_) (*-commutative y z) ⟩
  x * (z * y) ≡˘⟨ *-associative x z y ⟩
  x * z * y ∎
```
-->

Note that this representation, while convenient, does pose some problems.
We pay for the (relative) uniqueness by having larger terms: For instance, the
polynomial $X^4 + 1$ is represented as

```agda
private
  x⁴+1 : Poly Nat 1
  x⁴+1 = zerop *X+ const 1 *X+ const 0 *X+ const 0 *X+ const 0 *X+ const 0
```

This could be alleviated by using a *sparse* representation, but this is
decidedly more difficult. As the solver is not expected to deal with
polynomials with large degrees, this term blow-up will not be a problem
in practice.

### Operations on Horner normal forms

Now, let's define a handful of functions for constructing and combining
polynomials.  The naming here can get a bit confusing, so let's stick
with the convention of adding a subscript `p` to denote an operation on
polynomials. As a further note, the entire following section could be
generalized work over an arbitrary semiring, but this would complicate
the dependency graph somewhat, so we stick to natural numbers.

As previously mentioned, we have different representations of the $0$
polynomial depending on if we are working with `Poly A zero` or `Poly A
(suc n)`. This is somewhat annoying, so we define a small helper for
picking the correct representation.

```agda
0ₚ : Poly Nat n
0ₚ {n = zero}  = const zero
0ₚ {n = suc n} = zerop
```

While we are at it, we also define the polynomial that represents, given
a constant $c$, the constant polynomial $c \in A[X_0]\cdots[X_n]$.

```agda
constₚ : Nat → Poly Nat n
constₚ {n = zero}  c = const c
constₚ {n = suc n} c = 0ₚ *X+ constₚ c
```

The constant 1 is important enough that it deserves its own syntax.

```agda
1ₚ : Poly Nat n
1ₚ = constₚ 1
```

We also define the identity monomials $X_i \in A[X_0]\cdots[X_n]$.

```agda
X[_] : Fin n → Poly Nat n
X[ i ] with fin-view i
... | zero  = 1ₚ *X+ 0ₚ
... | suc i = 0ₚ *X+ X[ i ]
```

Now, onto addition of polynomials. This is more or less what one would
expect if they wrote out the polynomials and did the addition by hand.

```agda
infixl 6 _+ₚ_
infixl 7 _*ₚ_

_+ₚ_ : Poly Nat n → Poly Nat n → Poly Nat n
const c₁ +ₚ const c₂ = const (c₁ + c₂)
zerop +ₚ q = q
(p *X+ q) +ₚ zerop = p *X+ q
(p *X+ r) +ₚ (q *X+ s) = (p +ₚ q) *X+ (r +ₚ s)
```

Multiplication, however, is somewhat trickier. The problem is that
during the course of recursion, we will need to multiply a `Poly A n` by
a `Poly A (suc n)` --- for which we will need mutual recursion, since
that multiplication will fall back to the "homogeneous" case eventually.
We predeclare their types to make Agda happy:

```agda
_*ₚ_ : Poly Nat n → Poly Nat n → Poly Nat n
_*ₚ'_ : Poly Nat n → Poly Nat (suc n) → Poly Nat (suc n)
```

First, the homogeneous multiplication. The first two cases are pretty
straightforward, but the final one is decidedly less so. To start, we
can distribute the multiplication of `r` over the addition, invoking
`_+ₚ_`{.Agda} to add the results together. When multiplying `q` and `r`,
we need to use the aforementioned heterogeneous multiplication, as $q
\in A[X_1]\cdots[X_n]$ --- note that the index is off by one ($X_1$ vs
$X_0$). When multiplying `p` and `r`, we need to add on a `0ₚ` under the
`*X`, as this is the only way of multiplying by $X_0$.

```agda
const c₁  *ₚ const c₂ = const (c₁ * c₂)
zerop     *ₚ q        = zerop
(p *X+ q) *ₚ r        = ((p *ₚ r) *X+ 0ₚ) +ₚ (q *ₚ' r)
```

For the heterogeneous case, the call graph is simpler, as we can fall
back to the homogeneous operator.

```agda
r *ₚ' zerop     = zerop
r *ₚ' (p *X+ q) = (r *ₚ' p) *X+ (r *ₚ q)
```

### Evaluation of Horner normal forms

Multivariate polynomials represent functions $A^n \to A$, so we should
be able to interpret them as such. Luckily, Horner Normal Forms are
extremely easy to evaluate. As a historical note, this is why this
representation was created in first place! In this light, they should
probably be called "[Sharaf al-Din al-Tusi] normal forms".

[Sharaf al-Din al-Tusi]: https://en.wikipedia.org/wiki/Sharaf_al-Din_al-Tusi

```agda
block : Nat → Nat
block x = x
```

```agda
⟦_⟧ₚ : Poly Nat n → Vec Nat n → Nat
⟦ const c ⟧ₚ env        = c
⟦ zerop ⟧ₚ   env        = 0
⟦ p *X+ q ⟧ₚ (x₀ ∷ env) = ⟦ p ⟧ₚ (x₀ ∷ env) * x₀ + ⟦ q ⟧ₚ env
```

### Soundness of the operations

Now, it's important that the operations we defined actually denote the
correct operations on natural numbers. As a warm up, let's show that the
zero polynomial really represents the function $f(x_0, \cdots, x_n) =
0$.

```agda
sound-0ₚ : ∀ (env : Vec Nat n) → ⟦ 0ₚ ⟧ₚ env ≡ 0
sound-0ₚ []        = refl
sound-0ₚ (x ∷ env) = refl
```

We do the same for the constant polynomials:

```agda
sound-constₚ : ∀ c → (env : Vec Nat n) → ⟦ constₚ c ⟧ₚ env ≡ c
sound-constₚ c [] = refl
sound-constₚ c (x ∷ env) = sound-constₚ c env
```

At the risk of repeating ourselves, we also show the same for the
monomial $X_i$.

```agda
sound-X[_] : ∀ i → (env : Vec Nat n) → ⟦ X[ i ] ⟧ₚ env ≡ lookup env i
sound-X[ i ] _ with fin-view i
sound-X[ .fzero ] (x₀ ∷ env) | zero =
  ⟦ constₚ 1 ⟧ₚ env * x₀ + ⟦ 0ₚ ⟧ₚ env ≡⟨ ap₂ (λ ϕ ψ → ϕ * x₀ + ψ) (sound-constₚ 1 env) (sound-0ₚ env) ⟩
  1 * x₀ + 0                           ≡⟨ +-zeror (1 * x₀) ⟩
  1 * x₀                               ≡⟨ *-onel x₀ ⟩
  x₀ ∎
sound-X[ .(fsuc i) ] (_ ∷ env) | suc i = sound-X[ i ] env
```

Now, for something more involved: let's show that addition of
polynomials really deserves the name "addition" --- under the semantics
mapping `⟦_⟧ₚ`{.Agda}, adding two polynomials then evaluating is the
same thing as evaluating each then adding the results.

```agda
sound-+ₚ : ∀ p q → (env : Vec Nat n)
           → ⟦ p +ₚ q ⟧ₚ env ≡ ⟦ p ⟧ₚ env + ⟦ q ⟧ₚ env
sound-+ₚ (const c1) (const c2) env = refl
sound-+ₚ zerop q env = refl
sound-+ₚ (p *X+ r) zerop env =
  sym (+-zeror (⟦ (p *X+ r) +ₚ zerop ⟧ₚ env))
sound-+ₚ (p *X+ r) (q *X+ s) (x₀ ∷ env) =
  ⟦p+q⟧ * x₀ + ⟦r+s⟧                ≡⟨ ap₂ (λ ϕ ψ → ϕ * x₀ + ψ) (sound-+ₚ p q (x₀ ∷ env)) (sound-+ₚ r s env) ⟩
  (⟦p⟧ + ⟦q⟧) * x₀ + (⟦r⟧ + ⟦s⟧)    ≡⟨ ap (λ ϕ → ϕ + (⟦r⟧ + ⟦s⟧)) (*-distrib-+r ⟦p⟧ ⟦q⟧ x₀) ⟩
  ⟦p⟧ * x₀ + ⟦q⟧ * x₀ + (⟦r⟧ + ⟦s⟧) ≡⟨ commute-inner (⟦p⟧ * x₀) (⟦q⟧ * x₀) ⟦r⟧ ⟦s⟧ ⟩
  ⟦p⟧ * x₀ + ⟦r⟧ + (⟦q⟧ * x₀ + ⟦s⟧) ∎
  where
    ⟦p+q⟧ = ⟦ p +ₚ q ⟧ₚ (x₀ ∷ env)
    ⟦r+s⟧ = ⟦ r +ₚ s ⟧ₚ env
    ⟦p⟧ = ⟦ p ⟧ₚ (x₀ ∷ env)
    ⟦r⟧ = ⟦ r ⟧ₚ env
    ⟦q⟧ = ⟦ q ⟧ₚ (x₀ ∷ env)
    ⟦s⟧ = ⟦ s ⟧ₚ env
```

Wow, that was a bit painful! This is a common theme when writing proof
automation: it distills down a lot of the annoying proofs we need to
write across the entire code-base into one _extremely_ painful proof.
Thus, conservation of frustration is preserved.

Philosophical reflections aside, let's move onto multiplication of
polynomials.  As the homogeneous and heterogeneous multiplication were
defined in a mutually recursive manner, we must do so for their proofs
of soundness as well.

```agda
sound-*ₚ
  : ∀ p q → (env : Vec Nat n)
  → ⟦ p *ₚ q ⟧ₚ env ≡ ⟦ p ⟧ₚ env * ⟦ q ⟧ₚ env
sound-*ₚ'
  : ∀ p q → (x₀ : Nat) → (env : Vec Nat n)
  → ⟦ p *ₚ' q ⟧ₚ (x₀ ∷ env) ≡ ⟦ p ⟧ₚ env * ⟦ q ⟧ₚ (x₀ ∷ env)
```

The first couple of cases of homogeneous multiplication don't look so
bad...

```agda
sound-*ₚ (const c1) (const c2) env = refl
sound-*ₚ zerop q env = refl
sound-*ₚ (p *X+ r) zerop (x₀ ∷ env) =
  ⟦ p *ₚ zerop ⟧ₚ (x₀ ∷ env) * x₀ + ⟦ 0ₚ ⟧ₚ env ≡⟨ ap₂ (λ ϕ ψ → ϕ * x₀ + ψ) (sound-*ₚ p zerop (x₀ ∷ env)) (sound-0ₚ env) ⟩
  ⟦p⟧ * 0 * x₀ + 0                              ≡⟨ ap (λ ϕ → (ϕ * x₀) + 0) (*-zeror ⟦p⟧) ⟩
  0                                             ≡˘⟨ *-zeror (⟦p⟧ * x₀ + ⟦r⟧) ⟩
  (⟦p⟧ * x₀ + ⟦r⟧) * 0 ∎
  where
    ⟦p⟧ = ⟦ p ⟧ₚ (x₀ ∷ env)
    ⟦r⟧ = ⟦ r ⟧ₚ env
```

However, the case where we need to distribute is not so easy. The
consists of repeatedly expanding out the polynomial operations into
those on natural numbers, then doing a brutal bit of symbol shuffling.
There's not too much to be gained from dwelling on this, so let's move
on.

```agda
sound-*ₚ (p *X+ r) (q *X+ s) (x₀ ∷ env) =
  ⟦p*⟨qx+s⟩+r*q⟧ * x₀ + ⟦ 0ₚ +ₚ (r *ₚ s) ⟧ₚ env                ≡⟨ ap (λ ϕ → ⟦p*⟨qx+s⟩+r*q⟧ * x₀ + ϕ) (sound-+ₚ 0ₚ (r *ₚ s) env) ⟩
  ⟦p*⟨qx+s⟩+r*q⟧ * x₀ + (⟦ 0ₚ ⟧ₚ env + ⟦ r *ₚ s ⟧ₚ env)        ≡⟨ ap₂ (λ ϕ ψ → ⟦p*⟨qx+s⟩+r*q⟧ * x₀ + (ϕ + ψ)) (sound-0ₚ env) (sound-*ₚ r s env) ⟩
  ⟦p*⟨qx+s⟩+r*q⟧ * x₀ + (⟦r⟧ * ⟦s⟧)                            ≡⟨ ap (λ ϕ → ϕ * x₀ + ⟦r⟧ * ⟦s⟧) (sound-+ₚ (p *ₚ (q *X+ s)) (r *ₚ' q) (x₀ ∷ env)) ⟩
  (⟦p*⟨qx+s⟩⟧ + ⟦r*q⟧) * x₀ + ⟦r⟧ * ⟦s⟧                        ≡⟨ ap₂ (λ ϕ ψ → (ϕ + ψ) * x₀ + ⟦r⟧ * ⟦s⟧) (sound-*ₚ p (q *X+ s) (x₀ ∷ env)) (sound-*ₚ' r q x₀ env) ⟩
  (⟦p⟧ * (⟦q⟧ * x₀ + ⟦s⟧) + ⟦r⟧ * ⟦q⟧) * x₀ + ⟦r⟧ * ⟦s⟧        ≡⟨ ap (λ ϕ → ϕ + ⟦r⟧ * ⟦s⟧) (*-distrib-+r (⟦p⟧ * (⟦q⟧ * x₀ + ⟦s⟧)) (⟦r⟧ * ⟦q⟧) x₀) ⟩
  ⟦p⟧ * (⟦q⟧ * x₀ + ⟦s⟧) * x₀ + ⟦r⟧ * ⟦q⟧ * x₀ + ⟦r⟧ * ⟦s⟧     ≡˘⟨ +-associative (⟦p⟧ * (⟦q⟧ * x₀ + ⟦s⟧) * x₀) (⟦r⟧ * ⟦q⟧ * x₀) (⟦r⟧ * ⟦s⟧) ⟩
  ⟦p⟧ * (⟦q⟧ * x₀ + ⟦s⟧) * x₀ + (⟦r⟧ * ⟦q⟧ * x₀ + ⟦r⟧ * ⟦s⟧)   ≡⟨ ap (λ ϕ →  ⟦p⟧ * (⟦q⟧ * x₀ + ⟦s⟧) * x₀ + (ϕ + ⟦r⟧ * ⟦s⟧)) (*-associative ⟦r⟧ ⟦q⟧ x₀) ⟩
  ⟦p⟧ * (⟦q⟧ * x₀ + ⟦s⟧) * x₀ + (⟦r⟧ * (⟦q⟧ * x₀) + ⟦r⟧ * ⟦s⟧) ≡˘⟨ ap (λ ϕ → ⟦p⟧ * (⟦q⟧ * x₀ + ⟦s⟧) * x₀ + ϕ) (*-distrib-+l (⟦q⟧ * x₀) ⟦s⟧ ⟦r⟧) ⟩
  ⟦p⟧ * (⟦q⟧ * x₀ + ⟦s⟧) * x₀ + ⟦r⟧ * (⟦q⟧ * x₀ + ⟦s⟧)         ≡⟨ ap (λ ϕ → ϕ + ⟦r⟧ * (⟦q⟧ * x₀ + ⟦s⟧)) (commute-last ⟦p⟧ (⟦q⟧ * x₀ + ⟦s⟧) x₀) ⟩
  ⟦p⟧ * x₀ * (⟦q⟧ * x₀ + ⟦s⟧) + ⟦r⟧ * (⟦q⟧ * x₀ + ⟦s⟧)         ≡˘⟨ *-distrib-+r (⟦p⟧ * x₀) ⟦r⟧ (⟦q⟧ * x₀ + ⟦s⟧) ⟩
  (⟦p⟧ * x₀ + ⟦r⟧) * (⟦q⟧ * x₀ + ⟦s⟧)                          ∎
  where
    ⟦p*⟨qx+s⟩+r*q⟧ = ⟦ (p *ₚ (q *X+ s)) +ₚ (r *ₚ' q) ⟧ₚ (x₀ ∷ env)
    ⟦p*⟨qx+s⟩⟧ = ⟦ p *ₚ (q *X+ s) ⟧ₚ (x₀ ∷ env)
    ⟦r*q⟧ = ⟦ r *ₚ' q ⟧ₚ (x₀ ∷ env)
    ⟦p⟧ = ⟦ p ⟧ₚ (x₀ ∷ env)
    ⟦r⟧ = ⟦ r ⟧ₚ env
    ⟦q⟧ = ⟦ q ⟧ₚ (x₀ ∷ env)
    ⟦s⟧ = ⟦ s ⟧ₚ env
```

As a nice palate cleanser, the proofs for heterogeneous multiplication
are nowhere near as bad.

```agda
sound-*ₚ' p zerop x₀ env = sym (*-zeror (⟦ p ⟧ₚ env))
sound-*ₚ' r (p *X+ q) x₀ env =
  ⟦ r *ₚ' p ⟧ₚ (x₀ ∷ env) * x₀ + ⟦ r *ₚ q ⟧ₚ env ≡⟨ ap₂ (λ ϕ ψ → ϕ * x₀ + ψ) (sound-*ₚ' r p x₀ env) (sound-*ₚ r q env) ⟩
  ⟦r⟧ * ⟦p⟧ * x₀ + ⟦r⟧ * ⟦q⟧                     ≡⟨ ap (λ ϕ → ϕ + ⟦r⟧ * ⟦q⟧) (*-associative ⟦r⟧ ⟦p⟧ x₀) ⟩
  ⟦r⟧ * (⟦p⟧ * x₀) + ⟦r⟧ * ⟦q⟧                   ≡˘⟨ *-distrib-+l  (⟦p⟧ * x₀) ⟦q⟧ ⟦r⟧ ⟩
  ⟦r⟧ * (⟦p⟧ * x₀ + ⟦q⟧)                         ∎
  where
    ⟦r⟧ = ⟦ r ⟧ₚ env
    ⟦p⟧ = ⟦ p ⟧ₚ (x₀ ∷ env)
    ⟦q⟧ = ⟦ q ⟧ₚ env
```

This concludes phase one of the solver.

## Evaluation into polynomials

Now that we've gotten the first phase of the solver done, let's move on
to expressions in the language of natural numbers. Our first move shall
be defining expressions in the equational theory of natural numbers.

However, there is an efficiency problem we need to take care of here. If
we naively expand out `_+_`{.Agda} and `_*_`{.Agda} during reflection,
we could end up in a situation where we need to contend with a _huge_
amount of `suc`{.Agda} constructors when large literals get involved.
Therefore, we prevent reduction of such functions, but this means this
phase of the solver needs to be aware of nat literals.

With that in mind, let's define our expressions. Note that things that
the solver is unable to deal with (for instance, functions that aren't
`_+_`{.Agda} or `_*_`{.Agda}) are represented as variables, and will be
replaced during evaluation.

```agda
data Expr : Nat → Type where
  ‵0   : ∀ {n} → Expr n
  ‵lit : ∀ {n} → Nat    → Expr n
  ‵_   : ∀ {n} → Fin n  → Expr n
  ‵1+_ : ∀ {n} → Expr n → Expr n
  _‵+_ : ∀ {n} → Expr n → Expr n → Expr n
  _‵*_ : ∀ {n} → Expr n → Expr n → Expr n
```


We also define an interpretation of expressions into functions
$\mathbb{N}^n \to \mathbb{N}$.

```agda
⟦_⟧ₑ : Expr n → Vec Nat n → Nat
⟦ ‵ i      ⟧ₑ env = lookup env i
⟦ ‵0       ⟧ₑ env = 0
⟦ ‵1+ e    ⟧ₑ env = suc (⟦ e ⟧ₑ env)
⟦ ‵lit k   ⟧ₑ env = k
⟦ e1 ‵+ e2 ⟧ₑ env = ⟦ e1 ⟧ₑ env + ⟦ e2 ⟧ₑ env
⟦ e1 ‵* e2 ⟧ₑ env = ⟦ e1 ⟧ₑ env * ⟦ e2 ⟧ₑ env
```

We also define an evaluation of expressions into polynomials. The only
thing to note here is the evaluation of quoted `suc`{.Agda} constructors
as polynomial addition. This is somewhat inneficient, but in practice we
rarely have too many `suc`{.Agda} constructors to deal with, as we
handle literals separately.

```agda
↓_ : Expr n → Poly Nat n
↓ (‵ i)      = X[ i ]
↓ ‵0         = 0ₚ
↓ (‵1+ e)    = constₚ 1 +ₚ ↓ e
↓ ‵lit k     = constₚ k
↓ (e₁ ‵+ e₂) = (↓ e₁) +ₚ (↓ e₂)
↓ (e₁ ‵* e₂) = (↓ e₁) *ₚ (↓ e₂)
```

### Soundness of evaluation

With all of that machinery in place, our final proof shall be to show
that evaluating an expression into a polynomial has the same semantics
as the original expression. Luckily, most of the legwork is already
done, so we can sit back and enjoy the fruits of our labour.

```agda
sound : ∀ e → (env : Vec Nat n) → ⟦ ↓ e ⟧ₚ env ≡ ⟦ e ⟧ₑ env
sound (‵ i) env = sound-X[ i ] env
sound ‵0 env = sound-0ₚ env
sound (‵1+ e) env =
  ⟦ constₚ 1 +ₚ (↓ e) ⟧ₚ env       ≡⟨ sound-+ₚ (constₚ 1) (↓ e) env ⟩
  ⟦ constₚ 1 ⟧ₚ env + ⟦ ↓ e ⟧ₚ env ≡⟨ ap (λ ϕ → ϕ + ⟦ ↓ e ⟧ₚ env ) (sound-constₚ 1 env) ⟩
  suc (⟦ ↓ e ⟧ₚ env)               ≡⟨ ap suc (sound e env) ⟩
  suc (⟦ e ⟧ₑ env) ∎
sound (‵lit k) env = sound-constₚ k env
sound (e₁ ‵+ e₂) env =
  ⟦ (↓ e₁) +ₚ (↓ e₂) ⟧ₚ env     ≡⟨ sound-+ₚ (↓ e₁) (↓ e₂) env ⟩
  ⟦ ↓ e₁ ⟧ₚ env + ⟦ ↓ e₂ ⟧ₚ env ≡⟨ ap₂ _+_ (sound e₁ env) (sound e₂ env) ⟩
  ⟦ e₁ ⟧ₑ env + ⟦ e₂ ⟧ₑ env     ∎
sound (e₁ ‵* e₂) env =
  ⟦ (↓ e₁) *ₚ (↓ e₂) ⟧ₚ env     ≡⟨ sound-*ₚ (↓ e₁) (↓ e₂) env ⟩
  ⟦ ↓ e₁ ⟧ₚ env * ⟦ ↓ e₂ ⟧ₚ env ≡⟨ ap₂ _*_ (sound e₁ env) (sound e₂ env) ⟩
  ⟦ e₁ ⟧ₑ env * ⟦ e₂ ⟧ₑ env     ∎

```

Now, all we need to do is expose an interface for the reflection portion
of the solver. The `abstract` here is VERY IMPORTANT, as it prevents the
proof from unfolding into an enormous term that kills our compile
times.

```agda
abstract
  solve : ∀ e₁ e₂ → (env : Vec Nat n)
        → (⟦ ↓ e₁ ⟧ₚ env ≡ ⟦ ↓ e₂ ⟧ₚ env)
        → ⟦ e₁ ⟧ₑ env    ≡ ⟦ e₂ ⟧ₑ env
  solve e₁ e₂ env p = sym (sound e₁ env) ·· p ·· sound e₂ env
```

We also expose a function for "simplifying" expressions. In reality this
will almost always make the term more complicated, but it's useful for
debugging purposes.

```agda
expand : (e : Expr n) → (env : Vec Nat n) → Nat
expand e env = ⟦ ↓ e ⟧ₚ env
```

## Reflection

Now, for the _truly_ difficult part: the reflection interface. We begin
by defining some pattern synonyms for expressions we want to reflect
into our `Expr`{.Agda} type.

```agda
private
  pattern nat-lit n =
    def (quote Number.fromNat) (_ ∷ _ ∷ _ ∷ (lit (nat n)) v∷ _)
  pattern “zero” =
    con (quote Nat.zero) []
  pattern “suc” x =
    con (quote Nat.suc) (x v∷ [])
  pattern _“+”_ x y =
    def (quote _+_) (x v∷ y v∷ _)
  pattern _“*”_ x y =
    def (quote _*_) (x v∷ y v∷ _)
```

Next, we construct quoted a `Expr`{.Agda} from a term, replacing any
unknown `Term`{.Agda} nodes with variables. This uses the `Variable`
interface for managing the `Fin` variables and the environment. A
discussion of the internals of this is out of scope of this solver; we
have already looked into the abyss too deeply.

```agda
private
  build-expr : Variables Nat → Term → TC (Term × Variables Nat)
  build-expr vs (nat-lit n) = do
    ‵n ← quoteTC n
    pure $ con (quote ‵lit) (‵n v∷ []) , vs
  build-expr vs “zero” = do
    pure $ con (quote ‵0) (unknown h∷ []) , vs
  build-expr vs (“suc” t) = do
    e , vs ← build-expr vs t
    pure $ con (quote ‵1+_) (unknown h∷ e v∷ []) , vs
  build-expr vs (t₁ “+” t₂) = do
    e₁ , vs ← build-expr vs t₁
    e₂ , vs ← build-expr vs t₂
    pure $ con (quote _‵+_) (unknown h∷ e₁ v∷ e₂ v∷ []) , vs
  build-expr vs (t₁ “*” t₂) = do
    e₁ , vs ← build-expr vs t₁
    e₂ , vs ← build-expr vs t₂
    pure $ con (quote _‵*_) (unknown h∷ e₁ v∷ e₂ v∷ []) , vs
  build-expr vs tm = do
    (v , vs') ← bind-var vs tm
    pure $ con (quote ‵_) (v v∷ []) , vs'
```

Next, let's define the quoted forms of some terms that we will use to
interface with the solver.

```agda
private
  “expand” : Term → Term → Term
  “expand” e env = def (quote expand) (unknown h∷ e v∷ env v∷ [])

  “solve” : Term → Term → Term → Term
  “solve” lhs rhs env =
    def (quote solve)
        (unknown h∷ lhs v∷ rhs v∷ env v∷ def (quote refl) [] v∷ [])
```

### The actual macros

Now, the actual reflection API calls. In order to keep drawing this file
out, we start by defining some useful debugging macros. As we noted a
looong time ago, we don't want to unfold the `_+_`{.Agda} or
`_*_`{.Agda} functions, so let's make a list of those names so that we
can call `withReduceDefs`{.Agda} more easily.

```agda
private
  don't-reduce : List Name
  don't-reduce = quote _+_ ∷ quote _*_ ∷ quote Number.fromNat ∷ []
```

The `repr!` macro prints out a bunch of information about a given
expression of type `Nat`. This is _very_ useful when we are debugging.

```agda
repr-macro : Nat → Term → TC ⊤
repr-macro n hole =
  withNormalisation false $
  withReduceDefs (false , don't-reduce) $ do
  tm ← quoteTC n
  e , vs ← build-expr empty-vars tm
  size , env ← environment vs
  repr ← normalise $ def (quote ↓_) (size h∷ e v∷ [])
  typeError $ strErr "The expression\n  " ∷
                termErr tm ∷
              strErr "\nIs represented by the expression\n  " ∷
                termErr e ∷
              strErr "\nAnd the polynomial\n  " ∷
                termErr repr ∷
              strErr "\nThe environment is\n  " ∷
                termErr env ∷ []
macro
  repr! : Nat → Term → TC ⊤
  repr! n = repr-macro n
```

Slightly more useful is the `expand!` macro. This takes in a natural
number, and will fill in the hole with its expanded form. This is
intended to be used with the `agda2-elaborate-give` command in Emacs,
which is bound to `C-c RET` by default.

```agda
expand-macro : Nat → Term → TC ⊤
expand-macro n hole =
  withNormalisation false $
  withReduceDefs (false , don't-reduce) $ do
  tm ← quoteTC n
  e , vs ← build-expr empty-vars tm
  size , env ← environment vs
  expanded ← reduce (“expand” e env)
  unify hole expanded

macro
  expand! : Nat → Term → TC ⊤
  expand! n = expand-macro n
```

Now, finally, we have reached the summit. The `nat!` macro allows us
to automatically solve equations involving natural numbers.

```agda
solve-macro : Term → TC ⊤
solve-macro hole =
  withNormalisation false $
  withReduceDefs (false , don't-reduce) $ do
  goal ← infer-type hole >>= reduce

  just (lhs , rhs) ← get-boundary goal
    where nothing → typeError $ strErr "Can't determine boundary: " ∷
                                termErr goal ∷ []
  elhs , vs ← build-expr empty-vars lhs
  erhs , vs ← build-expr vs rhs
  size , env ← environment vs
  (noConstraints $ unify hole (“solve” elhs erhs env)) <|> do
    nf-lhs ← normalise (“expand” elhs env)
    nf-rhs ← normalise (“expand” erhs env)
    typeError (strErr "Could not solve the following goal:\n  " ∷
                 termErr lhs ∷ strErr " ≡ " ∷ termErr rhs ∷
               strErr "\nComputed normal forms:\n  LHS: " ∷
                 termErr nf-lhs ∷
               strErr "\n  RHS: " ∷
                 termErr nf-rhs ∷ [])

macro
  nat! : Term → TC ⊤
  nat! = solve-macro
```

# Examples

Congratulations! We now have a solver. Let's marvel at all of our hard
work for a moment.

```agda
private
  wow-good-job : ∀ x y z
               → (x + 5 + suc y) * z ≡ z * 5 + x * z + z + z * y
  wow-good-job x y z = nat!
```

Thus concludes our journey. There is still room for improvement,
however.  A sparse representation would be much more efficient, but
these proofs are already quite difficult to begin with. For the brave,
here is what a sparse representation might look like.

```agda
private
  data SparsePoly {a} (A : Type a) : Nat → Type a where
    const-sparse : ∀ {n} → A → SparsePoly A n
    shift        : ∀ {n} → (j : Nat) → SparsePoly A n
                   → SparsePoly A (j + n)
    _*X^_+_      : ∀ {n} → SparsePoly A (suc n) → Nat → SparsePoly A n
                   → SparsePoly A (suc n)
```
